Added documentation, readme.

Logic/Common/DynamicIndex.lean
@@ -1,32 +1,59 @@
 namespace Logic.DL
 
-inductive DynIdxSym where
-  | line : Nat → DynIdxSym
-  | hash : DynIdxSym
-  | dollar : DynIdxSym
+
+/--
+Inductive Type `DynIndexSym` modelling *the alphabet* Σ over which dynamic indices are built of.
+Dynamic index symbols are
+  • natural numbers       - modelling line numbers
+  • hash symbol #         - modelling termination
+  • dollar symbol $       - modelling iteration
+
+Dynamic index symbols serve as type for atomic relations in DA logic.
+Thus an atomic relation is either a natural number, # or $, but not a composed dynamic index.
+
+If Lean can't figure out that a natural number `n` is supposed to be a DynIndexSym, use the notation `ι n` for the line constructor.
+On the other hand, `ι i` can also be used to signify that `i` is specifically a line number (and not $ or #), so that e.g. `ι (i+1)` is a valid expression.
+-/
+inductive DynIndexSym where
+  | line : Nat → DynIndexSym                  -- line number n
+  | hash : DynIndexSym                        -- #
+  | dollar : DynIndexSym                      -- $
 deriving DecidableEq
 
+/--
+Inductive Type `DynIndex` modelling dynamic indices, i.e. words from Σ*, where Σ are dynamic index symbols, modelled by `DynIndexSym`
+
+Dynamic indices model program states in Executions and thus serve as states of the Kripke Model K_E associated with the execution E.
+Each dynamic index is prefixed by ε, i.e. the `root` in this model, after which dynamic index symbols can be concatened with the `cons` constructor.
+
+Notation for `root` is ε, for `cons` its `∘ᵢ`.
+
+Examples of dynamic indices:
+  • ε
+  • ε ∘ᵢ 0 ∘ᵢ 1 ∘ᵢ #
+  • ε ∘ᵢ $
+-/
 inductive DynIndex where
-  | root : DynIndex
-  | cons : DynIndex → DynIdxSym → DynIndex
+  | root : DynIndex                           -- ε
+  | cons : DynIndex → DynIndexSym → DynIndex  -- s ∘ᵢ i, where s is a dynamic index and i a dynamic index symbol
 deriving DecidableEq
 
 def line (ι: DynIndex) (n: Nat) :=
-  DynIndex.cons ι (DynIdxSym.line n)
+  DynIndex.cons ι (DynIndexSym.line n)
 
 def dollar (ι: DynIndex) :=
-  DynIndex.cons ι DynIdxSym.dollar
+  DynIndex.cons ι DynIndexSym.dollar
 
 def hash (ι: DynIndex) :=
-  DynIndex.cons ι DynIdxSym.hash
+  DynIndex.cons ι DynIndexSym.hash
 
-instance : Coe Nat DynIdxSym where
-  coe := DynIdxSym.line
+instance : Coe Nat DynIndexSym where
+  coe := DynIndexSym.line
 
 notation "ε" => DynIndex.root
-notation "$" => DynIdxSym.dollar
-notation "#" => DynIdxSym.hash
-notation "ι" => DynIdxSym.line
-infixl:80 "∘" => DynIndex.cons
+notation "$" => DynIndexSym.dollar
+notation "#" => DynIndexSym.hash
+notation "ι" => DynIndexSym.line
+infixl:80 "∘ᵢ" => DynIndex.cons
 
 end Logic.DL
