Main.lean
@@ -2,16 +2,87 @@ import Logic.Prop.Syntax
 import Logic.Prop.Semantics
 import Logic.DL.Syntax
 import Logic.DL.Semantics
---import Logic.DL.Notation
+import Logic.DL.Notation
 import Logic.DL.FinModelSemantics
 import Logic.REPEAT.Semantics
 
 
 def main : IO Unit := pure ()
 
+namespace GenericKripke
+open Logic.DL
+/- # Generic Dynamic Logic Example-/
+
+--atomic formulas
+inductive Atom
+  | p
+  | q
+deriving DecidableEq
+
+--atomic relations
+inductive RelAtom
+  | a
+  | b
+deriving DecidableEq
+
+
+--states
+inductive State
+  | s₀
+  | s₁
+  | s₂
+deriving DecidableEq
+
+def M : Logic.DL.KripkeModel RelAtom Atom State where
+  val
+    | .p, .s₀      => True    -- in s₀, p holds
+    | .q, .s₁      => True    -- in s₁, q holds
+    | .p, .s₂      => True    -- in s₂, p holds
+    | _, _         => False   -- no atomic proposition holds in another state
+  rel
+    | .a, .s₀, .s₁ => True    -- s₀ --a--> s₁
+    | .b, .s₁, .s₂ => True    -- s₁ --b--> s₂
+    | _, _, _      => False   -- no other transitions
+
+-- φ := ⟨a⟩q
+def φ : DLForm RelAtom Atom :=
+  DLForm.diamond (Relation.relAtom RelAtom.a) (DLForm.atom Atom.q)
+
+-- ψ := ⟨a ∪ b⟩¬p ∨ ¬q
+def ψ : DLForm RelAtom Atom :=
+  DLForm.diamond (Relation.comp (Relation.relAtom RelAtom.a) (Relation.relAtom RelAtom.b))
+    (disj (not (DLForm.atom Atom.p)) (not (DLForm.atom Atom.q)))
+
+-- M, s₀ ⊧ φ
+example : eval M φ State.s₀ := by
+  simp[M, φ, eval, evalRel]
+  use State.s₁
+
+-- M, s₀ ⊧ ψ
+example : eval M ψ State.s₀ := by
+  simp[M, ψ, eval, evalRel]
+  use State.s₂
+  constructor
+  · use State.s₁
+  · intro hp
+    intro hq
+    aesop
+
+-- two arbitrary atomic steps lead to s₂
+example : evalRel M (Relation.comp (Relation.wild) (Relation.wild)) State.s₀ State.s₂ := by
+  simp[evalRel, M]
+  use State.s₁
+  constructor
+  · use RelAtom.a
+  · use RelAtom.b
+
+end GenericKripke
+
+
 namespace Logic.DL
 
-def testQ : Set DynIndex := {ε, line ε 0, (line ε 0) ∘ #}
+/- # Execution Model -/
+def testQ : Set DynIndex := {ε, ε ∘ᵢ ι 0, (ε ∘ᵢ ι 0) ∘ᵢ #}
 def dummyProc : Proc := {
   id := 0,
   params := [],
@@ -41,9 +112,8 @@ def testExec : Execution := {
 }
 
 def M := executionModel testExec
-#check Logic.DL.DynIdxSym.line
-#check M.rel
-example : M.rel (Logic.DL.DynIdxSym.line 0) ε (line ε 0) := by
+
+example : M.rel (0) ε (ε ∘ᵢ ι 0) := by
   simp[M, executionModel]
   constructor
   · constructor
@@ -52,20 +122,12 @@ example : M.rel (Logic.DL.DynIdxSym.line 0) ε (line ε 0) := by
     left
     rfl
 
-#check (Logic.DL.evalRel M)
-
-#check (Logic.DL.evalRel M (Logic.DL.Relation.relAtom (Logic.DL.DynIdxSym.line 0)))
-
-#check (Logic.DL.evalRel M (Logic.DL.Relation.relAtom (Logic.DL.DynIdxSym.line 0)) DynIndex.root)
-
 example : Logic.DL.evalRel M
-                 (Logic.DL.Relation.comp
-                    (Logic.DL.Relation.relAtom (ι 0))
-                    (Logic.DL.Relation.relAtom #))
+                 (0 ∘ᵣ #)
                   ε
-                  ((line ε 0) ∘ #) := by
+                  ((ε ∘ᵢ ι 0) ∘ᵢ #) := by
   simp[Logic.DL.evalRel]
-  use (line ε 0)
+  use  (ε ∘ᵢ (ι 0))
   simp[M, executionModel]
   constructor
   · constructor
@@ -81,5 +143,27 @@ example : Logic.DL.evalRel M
     · right
       right
       constructor
+
+def φ : DAForm := ⟨0 ∪ 1*⟩ₗ "e" =ₑ "e"
+
+example : Logic.DL.eval M φ ε := by
+  simp[Logic.DL.eval, φ, M]
+  use (ε ∘ᵢ ι 0)
+  simp[Logic.DL.evalRel]
+  simp[executionModel]
+  constructor
+  · constructor
+    constructor
+    · left
+      rfl
+    · right
+      left
+      rfl
+  · constructor
+    · right
+      left
+      rfl
+    · unfold evalCond
+      rfl
 
 end Logic.DL
