Logic/Extension/Next.lean
@@ -1,0 +1,40 @@
+import Logic.REPEAT.Semantics
+import Logic.DL.Semantics
+
+open Logic.DL
+
+/- -/
+inductive RelAtomNext where
+  | dyn: DynIndexSym → RelAtomNext
+  | next: RelAtomNext
+deriving DecidableEq
+
+def executionModelNext (e: Execution) :
+  KripkeModel RelAtomNext Cond DynIndex where
+    val := (executionModel e).val
+    rel := λ a s₁ s₂ ↦
+      match a with
+        | .dyn i => (executionModel e).rel i s₁ s₂
+        | .next => (
+            (∃ u i,
+              s₁ = u ∘ᵢ ι i ∧
+              s₂ = u ∘ᵢ ι (i+1) ∧
+              s₂ ∈ e.quasi.cft.Q)
+            ∨
+            (∃ u i,
+              s₁ = u ∘ᵢ ι i ∧
+              (u ∘ᵢ ι (i+1) ∉ e.quasi.cft.Q) ∧
+              s₂ = u ∘ᵢ $ ∧
+              s₂ ∈ e.quasi.cft.Q)
+            ∨
+            (∃ u i,
+              s₁ = u ∘ᵢ ι i ∧
+              (u ∘ᵢ ι (i+1) ∉ e.quasi.cft.Q) ∧
+              (u ∘ᵢ $ ∉ e.quasi.cft.Q) ∧
+              s₂ = u ∘ᵢ # ∧
+              s₂ ∈ e.quasi.cft.Q)
+            ∨
+            (∃ u,
+              s₁ = u ∘ᵢ $ ∧
+              s₂ = u ∘ᵢ #)
+        )
