README.md
@@ -1,1 +1,88 @@
-# lean_examples
+# Mechanization of Dependent Assertion Logic in Lean
+
+This is a formalization of *Dependent Assertion Logic* (DA) in Lean, heavily based on "A semantic foundation for dependent assertion reasoning" by Dr. Lukas Grätz, 2026, unpublished; this paper is referenced in the following and in comments as "paper". 
+I sincerely recommend reading it to understand in particular the formalization approach of *REPEAT_arr* and the connection to dynamic logic.
+Relevant definitions are also referenced in the code when necessary.
+
+The project aims to mirror the paper definitions for DA as closely as possible to obtain a faithful formalization of DA in a theorem prover.
+The formalization is then used to verify semantic properties of DA as well as the soundness of tableau calculus rules (planned).
+
+## Installation
+
+Since the goal of this project is to develop proofs, you don't run anything in the classical sense of it.
+The primary way to explore the project and follow along proofs is therefore using the Lean 4 VSCodium extension and its interactive infoview, see https://lean-lang.org/install/
+
+### Prerequisites
+- Lean 4
+- Git
+- VSCodium/VSCode
+
+Simply clone the repository:
+```
+git clone TODO:URL
+cd TODO: repo name
+lake update
+lake build
+```
+This should automatically download both the required Lean version specified in lean-toolchain and the necessary Mathlib components.
+The Lean infoview on the right will then show you the current proof state interactively:
+![Infoview Screenshot](assets/infoview.png)
+## Features
+
+- generic dynamic logic semantics
+- executable semantics for finite kripke models
+- formalization of the REPEAT_arr programming language
+- instantiation of kripke models associated with valid REPEAT_arr executions
+- proofs of semantic properties of DA (wip)
+- soundness proofs of tableau calculus rules (planned)
+
+## Project Structure
+```
+Logic
+├── Common
+├── DL
+└── REPEAT
+
+Main.lean
+```
+### Module Overview
+- **Logic.Common** defines dynamic indices for execution states and atomic relations
+- **Logic.DL** defines generic syntax and semantics of dynamic logic, notation and executable finite model semantics
+- **Logic.REPEAT** defines the REPEAT_arr language, axiomatic execution semantics and constructs the necessary kripke models for DA evaluation
+- **Main.lean** showcases small examples
+
+
+## Design Differences
+Even though the formalization tries to mirror the paper very literally (which is why the axiomatic approach for REPEAT_arr semantics is chosen instead of inventing an operational semantics or similar), some things are conceptually different, e.g. to accomodate for Lean notation quirks or the formal type theory.
+
+### Notation
+Examples:
+| Concept | Paper  | Lean   |
+|---------------|--------|--------|
+| Dynamic Index | s i  | s ∘ᵢ i |
+| Dynamic Index | s #  | s ∘ᵢ # |
+| Dynamic Index | s 0  | s ∘ᵢ ι 0|
+| Relation      | s i  | s ∘ᵣ i |
+| Formula       | p ≤ q ∧ q ≤ p → p = q | "p" ≤ₑ "q" ∧ₗ "q" ≤ₑ "p" →ₗ "p" =ₑ "q" |
+| Formula       | ⟨0 ∪ 1*⟩ p = q | ⟨0 ∪ 1*⟩ₗ "p" =ₑ "q"|
+
+The most notable difference here are the indices, which are part of the operators to avoid clashes with built in Lean notation.
+You may read ∘ᵢ as dynamic index concatenation and ∘ᵣ as relation concatenation. The index ₗ on logical connectives is to distinguish it from Leans connectives (l standing for logic, since d or f have no unicode subscripts).
+The index ₑ serves a similar purpose for conditions (e for expressions, since also c has no unicode subscript).
+You can view any defined notation in the **Notation.lean** files in Logic.DL and Logic.Repeat and **Common/DynamicIndex.lean**.
+
+### Dynamic Indices
+Another notable difference is in the implementation of Dynamic Indices. The implementation distinguishes atomic dynamic indices, i.e. the alphabet Σ containing natural numbers n, $, # or the type **DynIndexSym**, from dynamic indices, i.e. words from Σ* or the type **DynIndex**.
+This does allow to instantiate the Atomic Relation type for DA with the type **DynIndexSym**, and as such atomic steps in a kripke model correspond directly to atomic dynamic indices.
+It also means that the concatenation of dynamic indices ∘ᵢ and the concatenation of relations ∘ᵣ are strictly distinguished other than in the paper.
+See **Common/DynamicIndex.lean** for implementation details.
+
+### Proofs
+In the **Logic/DL** and **Logic/REPEAT** respectively are also **Proof.lean** files, which contain a few basic proofs already (partially) developed.
+
+You can follow along proof states in the infoview when placing the cursor in the respective lines.
+
+Arguably the most interesting proofs so far are `assign_changes_exactly_one_cell`, which shows that after any assignment, exactly one array cell changed; another interesting one is `model_non_branching`, which varifies that any model induced by an execution is non branching.
+
+Further work on proofs include finishing the ones marked with `sorry` and various others - one idea for a future proof being that the axiomatic characterization of variable valuations determine a universal valuation exactly.
+### References
